added semantics for instructions 'ret void', 'lshr', 'and', 'or', 'malloc', 'free', 'zext', 'sext', 'icmp', 'select' and 'procedure'. We also defined 'bop' that includes 'and', 'or', 'lshr' and 'add'; 'ext' includes 'zext' and 'sext'; 'cast' includes 'inttoptr', 'ptrtoint', and 'bitcast'. These operations are the least subset of instructions that Softbound needs.
From 2.7, LLVM removed 'malloc' and 'free', and uses system builtin
malloc and free functions. I don't think this matters much. In our
memory model, we need to define their semantics anyway, so it doesn't
matter if they are supported instructions or functions in libraries.



git-svn-id: https://webdav.seas.upenn.edu/svn/sol/vol@2494 eef5ea85-cc2e-0410-bd84-0fae1f012da8

src/ssa/opsem_conv.v
@@ -178,27 +178,41 @@ Definition dbInsn__implies__dsop_plus_prop state state' tr (db:dbInsn state stat
   dsop_plus state state' tr.
 Definition dbop__implies__dsop_star_prop state state' tr (db:dbop state state' tr) := 
   dsop_star state state' tr.
-Definition dbFdef__implies__dsop_star_prop fid rt lp S TD Ps ECs lc gl Mem lc' gl' als' Mem' B'' Result tr 
-           (db:dbFdef fid rt lp S TD Ps ECs lc gl Mem lc' gl' als' Mem' B'' Result tr) := 
-  forall B' Is' la lb,
-  lookupFdefViaIDFromSystemC S fid = Some (fdef_intro (fheader_intro rt fid la) lb) ->
-  getEntryBlock (fdef_intro (fheader_intro rt fid la) lb) = Some B' ->
-  getEntryInsns B' = Some Is' ->
-  dsop_star
-    (mkState S TD Ps ((mkEC (fdef_intro (fheader_intro rt fid la) lb) 
-                             B' Is' (initLocals la (params2GVs TD lp lc gl))
-                            (params2GVs TD lp lc gl) nil)::ECs) gl Mem)
-    (mkState S TD Ps ((mkEC (fdef_intro (fheader_intro rt fid la) lb) 
-                             B'' ((insn_return rt Result)::nil) lc'
-                            (params2GVs TD lp lc gl) als')::ECs) gl' Mem')
-    tr
+Definition dbFdef__implies__dsop_star_prop fid rt lp S TD Ps ECs lc gl Mem lc' gl' als' Mem' B'' oResult tr 
+           (db:dbFdef fid rt lp S TD Ps ECs lc gl Mem lc' gl' als' Mem' B'' oResult tr) := 
+  match oResult with
+  | Some Result => forall B' Is' la lb,
+    lookupFdefViaIDFromSystemC S fid = Some (fdef_intro (fheader_intro rt fid la) lb) ->
+    getEntryBlock (fdef_intro (fheader_intro rt fid la) lb) = Some B' ->
+    getEntryInsns B' = Some Is' ->
+    dsop_star
+      (mkState S TD Ps ((mkEC (fdef_intro (fheader_intro rt fid la) lb) 
+                               B' Is' (initLocals la (params2GVs TD lp lc gl))
+                              (params2GVs TD lp lc gl) nil)::ECs) gl Mem)
+      (mkState S TD Ps ((mkEC (fdef_intro (fheader_intro rt fid la) lb) 
+                               B'' ((insn_return rt Result)::nil) lc'
+                              (params2GVs TD lp lc gl) als')::ECs) gl' Mem')
+      tr
+  | None => forall B' Is' la lb,
+    lookupFdefViaIDFromSystemC S fid = Some (fdef_intro (fheader_intro rt fid la) lb) ->
+    getEntryBlock (fdef_intro (fheader_intro rt fid la) lb) = Some B' ->  
+    getEntryInsns B' = Some Is' ->
+    dsop_star
+      (mkState S TD Ps ((mkEC (fdef_intro (fheader_intro rt fid la) lb) 
+                               B' Is' (initLocals la (params2GVs TD lp lc gl))
+                              (params2GVs TD lp lc gl) nil)::ECs) gl Mem)
+      (mkState S TD Ps ((mkEC (fdef_intro (fheader_intro rt fid la) lb) 
+                               B'' ((insn_return_void)::nil) lc'
+                              (params2GVs TD lp lc gl) als')::ECs) gl' Mem')
+      tr
+  end
   .
 
 Lemma db__implies__ds:
   (forall state state' t  db, @dbInsn__implies__dsop_plus_prop state state' t db) /\
   (forall state state' t  db, @dbop__implies__dsop_star_prop state state' t db) /\
-  (forall fid rt lp S TD Ps ECs lc gl Mem lc' gl' als' Mem' B'' ret tr db, 
-     @dbFdef__implies__dsop_star_prop fid rt lp S TD Ps ECs lc gl Mem lc' gl' als' Mem' B'' ret tr db).
+  (forall fid rt lp S TD Ps ECs lc gl Mem lc' gl' als' Mem' B'' oret tr db, 
+     @dbFdef__implies__dsop_star_prop fid rt lp S TD Ps ECs lc gl Mem lc' gl' als' Mem' B'' oret tr db).
 Proof.
 (db_mutind_cases
   apply db_mutind with
@@ -210,8 +224,9 @@ Proof.
          dbop__implies__dsop_star_prop, 
          dbFdef__implies__dsop_star_prop; 
   intros; subst; simpl; intuition; eauto.
-  Case "dbCallInsn".
-    inversion d. subst.
+  Case "dbCall".
+    inversion d; subst.
+    SCase "dbFdef_func".
     assert (Hlookup:=H0).
     apply H with (B'0:=B'0)(Is':=Is') in H0; auto.
     rewrite <- nil_app_trace__eq__trace.
@@ -219,22 +234,46 @@ Proof.
       (state2:=mkState S TD Ps ((mkEC (fdef_intro (fheader_intro rt fid la) lb)
                                B'0 Is' (initLocals la (params2GVs TD lp lc gl)) 
                                (params2GVs TD lp lc gl) nil)::
-                        (mkEC F B ((insn_call rid rt fid lp)::Is) lc arg als)::EC) 
+                        (mkEC F B ((insn_call orid tailc rt fid lp)::Is) lc arg als)::EC) 
                         gl Mem); auto.
     rewrite <- trace_app_nil__eq__trace.
     apply dsop_star_trans with 
       (state2:=mkState S TD Ps ((mkEC (fdef_intro (fheader_intro rt fid la) lb) 
                                B' ((insn_return rt Result)::nil) lc'
                                (params2GVs TD lp lc gl) als')::
-                        (mkEC F B ((insn_call rid rt fid lp)::Is) lc arg als)::EC) 
+                        (mkEC F B ((insn_call orid tailc rt fid lp)::Is) lc arg als)::EC) 
                         gl' Mem'); auto.
-      apply dsInsn__implies__dsop_star.
-      eapply dsReturn; simpl; eauto.
-  
+
+    SCase "dbFdef_proc".
+    assert (Hlookup:=H0).
+    apply H with (B'0:=B'0)(Is':=Is') in H0; auto.
+    rewrite <- nil_app_trace__eq__trace.
+    apply dsop_plus_cons with 
+      (state2:=mkState S TD Ps ((mkEC (fdef_intro (fheader_intro rt fid la) lb)
+                               B'0 Is' (initLocals la (params2GVs TD lp lc gl)) 
+                               (params2GVs TD lp lc gl) nil)::
+                        (mkEC F B ((insn_call orid tailc rt fid lp)::Is) lc arg als)::EC) 
+                        gl Mem); auto.
+    rewrite <- trace_app_nil__eq__trace.
+    apply dsop_star_trans with 
+      (state2:=mkState S TD Ps ((mkEC (fdef_intro (fheader_intro rt fid la) lb) 
+                               B' ((insn_return_void)::nil) lc'
+                               (params2GVs TD lp lc gl) als')::
+                        (mkEC F B ((insn_call orid tailc rt fid lp)::Is) lc arg als)::EC) 
+                        gl' Mem'); auto.
+      destruct orid; try solve [inversion e; subst; auto].
+      destruct (rt =t= typ_void); try solve [inversion e; subst; auto].
+
   Case "dbop_cons".
     apply dsop_star_trans with (state2:=S2); auto.
         
-  Case "dbFdef_intro".
+  Case "dbFdef_func".
+    rewrite H0 in e. inversion e; subst.
+    rewrite H1 in e0. inversion e0; subst.
+    rewrite H2 in e1. inversion e1; subst.
+    exact H.
+
+  Case "dbFdef_proc".
     rewrite H0 in e. inversion e; subst.
     rewrite H1 in e0. inversion e0; subst.
     rewrite H2 in e1. inversion e1; subst.
@@ -263,8 +302,8 @@ Proof.
   destruct db__implies__ds as [_ [J _]]. eauto.
 Qed.
 
-Lemma dbFdef__implies__dsop_star : forall fid rt lp S TD Ps ECs lc gl Mem lc' gl' als' Mem' B'' Result tr B' Is' la lb,
-  dbFdef fid rt lp S TD Ps ECs lc gl Mem lc' gl' als' Mem' B'' Result tr ->
+Lemma dbFdef_func__implies__dsop_star : forall fid rt lp S TD Ps ECs lc gl Mem lc' gl' als' Mem' B'' Result tr B' Is' la lb,
+  dbFdef fid rt lp S TD Ps ECs lc gl Mem lc' gl' als' Mem' B'' (Some Result) tr ->
   lookupFdefViaIDFromSystemC S fid = Some (fdef_intro (fheader_intro rt fid la) lb) ->
   getEntryBlock (fdef_intro (fheader_intro rt fid la) lb) = Some B' ->
   getEntryInsns B' = Some Is' ->
@@ -277,9 +316,28 @@ Lemma dbFdef__implies__dsop_star : forall fid rt lp S TD Ps ECs lc gl Mem lc' gl
                             (params2GVs TD lp lc gl) als')::ECs) gl' Mem')
     tr.
 Proof.
-  intros fid rt lp S TD Ps EC lc gl Mem lc' gl' als' Mem' B'' Result tr B' Is' la lb H.
-  revert fid rt lp S TD Ps EC lc gl Mem lc' gl' als' Mem' B'' Result tr H B' Is' la lb.
-  destruct db__implies__ds as [_ [_ J]]. eauto.
+  intros fid rt lp S TD Ps EC lc gl Mem lc' gl' als' Mem' B'' Result tr B' Is' la lb H H1 H2 H3.
+  destruct db__implies__ds as [_ [_ J]]. 
+  assert (K:=@J fid rt lp S TD Ps EC lc gl Mem lc' gl' als' Mem' B'' (Some Result) tr H B' Is' la lb H1 H2 H3); auto.
+Qed.
+
+Lemma dbFdef_proc__implies__dsop_star : forall fid rt lp S TD Ps ECs lc gl Mem lc' gl' als' Mem' B'' tr B' Is' la lb,
+  dbFdef fid rt lp S TD Ps ECs lc gl Mem lc' gl' als' Mem' B'' None tr ->
+  lookupFdefViaIDFromSystemC S fid = Some (fdef_intro (fheader_intro rt fid la) lb) ->
+  getEntryBlock (fdef_intro (fheader_intro rt fid la) lb) = Some B' ->
+  getEntryInsns B' = Some Is' ->
+  dsop_star 
+    (mkState S TD Ps ((mkEC (fdef_intro (fheader_intro rt fid la) lb) 
+                             B' Is' (initLocals la (params2GVs TD lp lc gl))
+                            (params2GVs TD lp lc gl) nil)::ECs) gl Mem)
+    (mkState S TD Ps ((mkEC (fdef_intro (fheader_intro rt fid la) lb) 
+                             B'' ((insn_return_void)::nil) lc'
+                            (params2GVs TD lp lc gl) als')::ECs) gl' Mem')
+    tr.
+Proof.
+  intros fid rt lp S TD Ps EC lc gl Mem lc' gl' als' Mem' B'' tr B' Is' la lb H H1 H2 H3.
+  destruct db__implies__ds as [_ [_ J]]. 
+  assert (K:=@J fid rt lp S TD Ps EC lc gl Mem lc' gl' als' Mem' B'' None tr H B' Is' la lb H1 H2 H3); auto.
 Qed.
 
 (** Then we prove that the whole program holds the same property. *)
@@ -337,7 +395,7 @@ Proof.
       (state2:=mkState S TD Ps ((mkEC (fdef_intro (fheader_intro rt fid la) lb)
                                B' Is' (initLocals la (params2GVs TD lp lc gl)) 
                                (params2GVs TD lp lc gl) nil)::
-                        (mkEC F B ((insn_call rid rt fid lp)::Is) lc arg als)::EC) 
+                        (mkEC F B ((insn_call rid tailc rt fid lp)::Is) lc arg als)::EC) 
                         gl Mem); 
       try solve [clear CIH_dbFdefInf CIH_dbInsnInf; auto].
       apply CIH_dbFdefInf with (B':=B')(Is':=Is')(la:=la)(lb:=lb) in HdbFdefInf; auto.
@@ -381,7 +439,7 @@ Proof.
     (state2:=mkState S TD Ps ((mkEC (fdef_intro (fheader_intro rt fid la) lb)
                              B' Is' (initLocals la (params2GVs TD lp lc gl)) 
                              (params2GVs TD lp lc gl) nil)::
-                      (mkEC F B ((insn_call rid rt fid lp)::Is) lc arg als)::EC) 
+                      (mkEC F B ((insn_call rid tailc rt fid lp)::Is) lc arg als)::EC) 
                       gl Mem); 
     try solve [clear CIH_dbInsnInf; auto].
     apply dbFdefInf__implies__dsop_diverges with (B':=B')(Is':=Is')(la:=la)(lb:=lb) in HdbFdefInf; auto.
@@ -425,8 +483,8 @@ Definition nbInsn__implies__nsop_plus_prop state_tr states' (nb:nbInsn state_tr 
   nsop_plus (state_tr::nil) states'.
 Definition nbop_star__implies__nsop_star_prop states states' (nb:nbop_star states states') := 
   nsop_star states states'.
-Definition nbFdef__implies__nsop_star_prop fid rt lp S TD Ps ECs lc gl Mem tr lc_gl_als_Mem_block_re_trs 
-           (nb:nbFdef fid rt lp S TD Ps ECs lc gl Mem tr lc_gl_als_Mem_block_re_trs) := 
+Definition nbFdef__implies__nsop_star_prop fid rt lp S TD Ps ECs lc gl Mem tr lc_gl_als_Mem_block_ore_trs 
+           (nb:nbFdef fid rt lp S TD Ps ECs lc gl Mem tr lc_gl_als_Mem_block_ore_trs) := 
   forall B' Is' la lb,
   lookupFdefViaIDFromSystemC S fid = Some (fdef_intro (fheader_intro rt fid la) lb) ->
   getEntryBlock (fdef_intro (fheader_intro rt fid la) lb) = Some B' ->
@@ -435,23 +493,23 @@ Definition nbFdef__implies__nsop_star_prop fid rt lp S TD Ps ECs lc gl Mem tr lc
     ((mkState S TD Ps ((mkEC (fdef_intro (fheader_intro rt fid la) lb) 
                              B' Is' (initLocals la (params2GVs TD lp lc gl))
                             (params2GVs TD lp lc gl) nil)::ECs) gl Mem, tr)::nil)
-    (returnStatesFromOp S TD Ps ECs lp lc gl rt fid la lb lc_gl_als_Mem_block_re_trs)
+    (returnStatesFromOp S TD Ps ECs lp lc gl rt fid la lb lc_gl_als_Mem_block_ore_trs)
   .
 
 Lemma returnStatesFromOp__nsop_star__updateStatesFromReturns : 
-forall lc_gl_als_Mem_block_re_trs S TD Ps F B rid (rt:typ) (fid:id) lp
+forall lc_gl_als_Mem_block_ore_trs S TD Ps F B orid tailc (rt:typ) (fid:id) lp
        (lc:GVMap) arg als EC Is lc gl rt fid la lb states,
-  updateStatesFromReturns S TD Ps F B Is lc rt arg als EC rid lc_gl_als_Mem_block_re_trs = Some states ->
+  updateStatesFromReturns S TD Ps F B Is lc rt arg als EC orid lc_gl_als_Mem_block_ore_trs = Some states ->
   nsop_star
-    (returnStatesFromOp S TD Ps (mkEC F B ((insn_call rid rt fid lp)::Is) lc arg als::EC)
-                        lp lc gl rt fid la lb lc_gl_als_Mem_block_re_trs)
+    (returnStatesFromOp S TD Ps (mkEC F B ((insn_call orid tailc rt fid lp)::Is) lc arg als::EC)
+                        lp lc gl rt fid la lb lc_gl_als_Mem_block_ore_trs)
     states.
 Proof.
-  induction lc_gl_als_Mem_block_re_trs; simpl; intros.
+  induction lc_gl_als_Mem_block_ore_trs; simpl; intros.
   inversion H; subst; auto.
 
   destruct a as [p tr]. 
-  destruct p as [p re]. 
+  destruct p as [p ore]. 
   destruct p as [p B'']. 
   destruct p as [p Mem']. 
   destruct p as [p als'].
@@ -459,36 +517,118 @@ Proof.
   remember (rt0 =t= typ_void) as rt0_eq_void.
   destruct rt0_eq_void.
   Case "rt0_is_void".
-    remember (free_allocas Mem' als') as Mem''.
-    destruct Mem''; simpl in H; try solve [inversion H; subst].
-    remember (updateStatesFromReturns S TD Ps F B Is lc0 rt0 arg als EC rid lc_gl_als_Mem_block_re_trs) as states2.
-    destruct states2; simpl in H; inversion H; subst.
-    assert (
-      (mkState S TD Ps (mkEC F B Is lc0 arg als::EC) gl' m, tr)::s = 
-      ((mkState S TD Ps (mkEC F B Is lc0 arg als::EC) gl' m, tr)::nil) ++ s
-    ) as EQ. auto.
-    rewrite EQ.
-    apply nsop_star_cons; auto.
-      rewrite app_nil_end.
-      eapply nsReturn; simpl; eauto.
-        rewrite <- Heqrt0_eq_void. auto.
+   destruct ore as [ re | ].
+   SCase "ore = Some re".    
+    destruct orid as [ rid | ].
+    SSCase "orid = Some rid".
+      remember (free_allocas Mem' als') as Mem''.
+      destruct Mem''; simpl in H; try solve [inversion H; subst].
+      remember (updateStatesFromReturns S TD Ps F B Is lc0 rt0 arg als EC (Some rid) lc_gl_als_Mem_block_ore_trs) as states2.
+      destruct states2; simpl in H; inversion H; subst.
+      assert (
+        (mkState S TD Ps (mkEC F B Is lc0 arg als::EC) gl' m, tr)::s = 
+        ((mkState S TD Ps (mkEC F B Is lc0 arg als::EC) gl' m, tr)::nil) ++ s
+      ) as EQ. auto.
+      rewrite EQ.
+      apply nsop_star_cons; auto.
+        rewrite app_nil_end.
+        eapply nsReturn; simpl; eauto.
+          rewrite <- Heqrt0_eq_void. auto.
+    SSCase "orid = None".
+      remember (free_allocas Mem' als') as Mem''.
+      destruct Mem''; simpl in H; try solve [inversion H; subst].
+      remember (updateStatesFromReturns S TD Ps F B Is lc0 rt0 arg als EC None lc_gl_als_Mem_block_ore_trs) as states2.
+      destruct states2; simpl in H; inversion H; subst.
+      assert (
+        (mkState S TD Ps (mkEC F B Is lc0 arg als::EC) gl' m, tr)::s = 
+        ((mkState S TD Ps (mkEC F B Is lc0 arg als::EC) gl' m, tr)::nil) ++ s
+      ) as EQ. auto.
+      rewrite EQ.
+      apply nsop_star_cons; auto.
+   SCase "ore = None".    
+    destruct orid as [ rid | ].
+    SSCase "orid = Some rid".
+      remember (free_allocas Mem' als') as Mem''.
+      destruct Mem''; simpl in H; try solve [inversion H; subst].
+      remember (updateStatesFromReturns S TD Ps F B Is lc0 rt0 arg als EC (Some rid) lc_gl_als_Mem_block_ore_trs) as states2.
+      destruct states2; simpl in H; inversion H; subst.
+      assert (
+        (mkState S TD Ps (mkEC F B Is lc0 arg als::EC) gl' m, tr)::s = 
+        ((mkState S TD Ps (mkEC F B Is lc0 arg als::EC) gl' m, tr)::nil) ++ s
+      ) as EQ. auto.
+      rewrite EQ.
+      apply nsop_star_cons; auto.
+    SSCase "orid = None".
+      remember (free_allocas Mem' als') as Mem''.
+      destruct Mem''; simpl in H; try solve [inversion H; subst].
+      remember (updateStatesFromReturns S TD Ps F B Is lc0 rt0 arg als EC None lc_gl_als_Mem_block_ore_trs) as states2.
+      destruct states2; simpl in H; inversion H; subst.
+      assert (
+        (mkState S TD Ps (mkEC F B Is lc0 arg als::EC) gl' m, tr)::s = 
+        ((mkState S TD Ps (mkEC F B Is lc0 arg als::EC) gl' m, tr)::nil) ++ s
+      ) as EQ. auto.
+      rewrite EQ.
+      apply nsop_star_cons; auto.
 
   Case "rt0_isnt_void".
-    remember (updateEnv lc0 gl' rid (getOperandValue TD re lc' gl')) as lc_gl.
-    destruct lc_gl as [lc'' gl''].
-    remember (free_allocas Mem' als') as Mem''.
-    destruct Mem''; simpl in H; try solve [inversion H; subst].
-    remember (updateStatesFromReturns S TD Ps F B Is lc0 rt0 arg als EC rid lc_gl_als_Mem_block_re_trs) as states2.
-    destruct states2; simpl in H; inversion H; subst.
-    assert (
-      (mkState S TD Ps (mkEC F B Is lc'' arg als::EC) gl'' m, tr)::s = 
-      ((mkState S TD Ps (mkEC F B Is lc'' arg als::EC) gl'' m, tr)::nil) ++ s
-    ) as EQ. auto.
-    rewrite EQ.
-    apply nsop_star_cons; auto.
-      rewrite app_nil_end.
-      eapply nsReturn; simpl; eauto.
-        rewrite <- Heqrt0_eq_void. auto.
+   destruct ore as [ re | ].
+   SCase "ore = Some re".    
+    destruct orid as [ rid | ].
+    SSCase "orid = Some rid".
+      remember (updateEnv lc0 gl' rid (getOperandValue TD re lc' gl')) as lc_gl.  
+      destruct lc_gl as [lc'' gl''].
+      remember (free_allocas Mem' als') as Mem''.
+      destruct Mem''; simpl in H; try solve [inversion H; subst].
+      remember (updateStatesFromReturns S TD Ps F B Is lc0 rt0 arg als EC (Some rid) lc_gl_als_Mem_block_ore_trs) as states2.
+      destruct states2; simpl in H; inversion H; subst.
+      assert (
+        (mkState S TD Ps (mkEC F B Is lc'' arg als::EC) gl'' m, tr)::s = 
+        ((mkState S TD Ps (mkEC F B Is lc'' arg als::EC) gl'' m, tr)::nil) ++ s
+      ) as EQ. auto.
+      rewrite EQ.
+      apply nsop_star_cons; auto.
+        rewrite app_nil_end.
+        eapply nsReturn; simpl; eauto.
+          rewrite <- Heqrt0_eq_void. auto.
+    SSCase "orid = None".
+      remember (free_allocas Mem' als') as Mem''.
+      destruct Mem''; simpl in H; try solve [inversion H; subst].
+      remember (updateStatesFromReturns S TD Ps F B Is lc0 rt0 arg als EC None lc_gl_als_Mem_block_ore_trs) as states2.
+      destruct states2; simpl in H; inversion H; subst.
+      assert (
+        (mkState S TD Ps (mkEC F B Is lc0 arg als::EC) gl' m, tr)::s = 
+        ((mkState S TD Ps (mkEC F B Is lc0 arg als::EC) gl' m, tr)::nil) ++ s
+      ) as EQ. auto.
+      rewrite EQ.
+      apply nsop_star_cons; auto.
+   SCase "ore = None".    
+    destruct orid as [ rid | ].
+    SSCase "orid = Some rid".
+      remember (free_allocas Mem' als') as Mem''.
+      destruct Mem''; simpl in H; try solve [inversion H; subst].
+      remember (updateStatesFromReturns S TD Ps F B Is lc0 rt0 arg als EC (Some rid) lc_gl_als_Mem_block_ore_trs) as states2.
+      destruct states2; simpl in H; inversion H; subst.
+      assert (
+        (mkState S TD Ps (mkEC F B Is lc0 arg als::EC) gl' m, tr)::s = 
+        ((mkState S TD Ps (mkEC F B Is lc0 arg als::EC) gl' m, tr)::nil) ++ s
+      ) as EQ. auto.
+      rewrite EQ.
+      apply nsop_star_cons; auto.
+        rewrite app_nil_end.
+    SSCase "orid = None".
+      remember (free_allocas Mem' als') as Mem''.
+      destruct Mem''; simpl in H; try solve [inversion H; subst].
+      remember (updateStatesFromReturns S TD Ps F B Is lc0 rt0 arg als EC None lc_gl_als_Mem_block_ore_trs) as states2.
+      destruct states2; simpl in H; inversion H; subst.
+      assert (
+        ((mkState S TD Ps (mkEC F B Is lc0 arg als::EC) gl' m, tr)::s) ++ nil = 
+        ((mkState S TD Ps (mkEC F B Is lc0 arg als::EC) gl' m, tr)::nil) ++ s
+      ) as EQ.
+        rewrite <- app_comm_cons.
+        rewrite <- app_comm_cons.
+        rewrite app_nil_end. auto.
+      rewrite EQ.
+      apply nsop_star_cons; eauto.
 Qed.
 
 Lemma nb__implies__ns:
@@ -524,6 +664,15 @@ Proof.
   Case "nbBranch_uncond".
     apply nsop_plus_trans with (states2:=(mkState S TD Ps (mkEC F B' Is' lc' arg als::EC) gl Mem, tr)::nil); auto.
       rewrite app_nil_end; eauto.
+  Case "nbMalloc".
+    apply nsop_plus_trans with (states2:=(mkState S TD Ps (mkEC F B Is lc' arg als::EC) gl' Mem', tr)::nil); auto.
+      rewrite app_nil_end; eauto.
+  Case "nbFree".
+    apply nsop_plus_trans with (states2:=(mkState S TD Ps (mkEC F B Is lc arg als::EC) gl Mem', tr)::nil); auto.
+      rewrite app_nil_end; eauto.
+  Case "nbAlloca".
+    apply nsop_plus_trans with (states2:=(mkState S TD Ps (mkEC F B Is lc' arg (mb::als)::EC) gl' Mem', tr)::nil); auto.
+      rewrite app_nil_end; eauto.
   Case "nbCall".
     inversion n. subst.
     assert (Hlookup:=H0).
@@ -532,17 +681,14 @@ Proof.
       (states2:=(mkState S TD Ps ((mkEC (fdef_intro (fheader_intro rt fid la) lb)
                                B' Is' (initLocals la (params2GVs TD lp lc gl)) 
                                (params2GVs TD lp lc gl) nil)::
-                              (mkEC F B ((insn_call rid rt fid lp)::Is) lc arg als)::EC) 
+                              (mkEC F B ((insn_call orid tailc rt fid lp)::Is) lc arg als)::EC) 
                                gl Mem, tr)::nil); auto.
       rewrite app_nil_end; eauto.
 
       apply nsop_star_trans with 
-        (states2:=returnStatesFromOp S TD Ps (mkEC F B ((insn_call rid rt fid lp)::Is) lc arg als::EC)
-                              lp lc gl rt fid la lb lc_gl_als_Mem_block_re_trs); auto.
+        (states2:=returnStatesFromOp S TD Ps (mkEC F B ((insn_call orid tailc rt fid lp)::Is) lc arg als::EC)
+                              lp lc gl rt fid la lb lc_gl_als_Mem_block_ore_trs); auto.
       apply returnStatesFromOp__nsop_star__updateStatesFromReturns with (Is:=Is); auto.
-  Case "nbAlloca".
-    apply nsop_plus_trans with (states2:=(mkState S TD Ps (mkEC F B Is lc' arg (mb::als)::EC) gl' Mem', tr)::nil); auto.
-      rewrite app_nil_end; eauto.
 
   Case "nbop_star_cons".
     assert ((state, tr)::states=((state, tr)::nil)++states) as EQ. auto.
@@ -667,13 +813,13 @@ Proof.
       (states':=(mkState S TD Ps ((mkEC (fdef_intro (fheader_intro rt fid la) lb)
                                B' Is' (initLocals la (params2GVs TD lp lc gl)) 
                                (params2GVs TD lp lc gl) nil)::
-                        (mkEC F B ((insn_call rid rt fid lp)::Is) lc arg als)::EC) 
+                        (mkEC F B ((insn_call rid tailc rt fid lp)::Is) lc arg als)::EC) 
                         gl Mem, tr)::nil).
       apply nsop_plus_trans 
         with (states2:=(mkState S TD Ps ((mkEC (fdef_intro (fheader_intro rt fid la) lb)
                                          B' Is' (initLocals la (params2GVs TD lp lc gl)) 
                                          (params2GVs TD lp lc gl) nil)::
-                                     (mkEC F B ((insn_call rid rt fid lp)::Is) lc arg als)::EC) 
+                                     (mkEC F B ((insn_call rid tailc rt fid lp)::Is) lc arg als)::EC) 
                                      gl Mem, tr)::nil); auto.
         rewrite app_nil_end; eauto.
       
@@ -716,13 +862,13 @@ Proof.
     (states':=(mkState S TD Ps ((mkEC (fdef_intro (fheader_intro rt fid la) lb)
                              B' Is' (initLocals la (params2GVs TD lp lc gl)) 
                              (params2GVs TD lp lc gl) nil)::
-                      (mkEC F B ((insn_call rid rt fid lp)::Is) lc arg als)::EC) 
+                      (mkEC F B ((insn_call rid tailc rt fid lp)::Is) lc arg als)::EC) 
                       gl Mem, tr)::nil).
     apply nsop_plus_trans 
       with (states2:=(mkState S TD Ps ((mkEC (fdef_intro (fheader_intro rt fid la) lb)
                                        B' Is' (initLocals la (params2GVs TD lp lc gl)) 
                                        (params2GVs TD lp lc gl) nil)::
-                                   (mkEC F B ((insn_call rid rt fid lp)::Is) lc arg als)::EC) 
+                                   (mkEC F B ((insn_call rid tailc rt fid lp)::Is) lc arg als)::EC) 
                                    gl Mem, tr)::nil); auto.
       rewrite app_nil_end; eauto.
     
